Debug netlist generation

Pkg.hs
@@ -1,0 +1,592 @@
+
+{-# OPTIONS_GHC -cpp -XMagicHash #-}
+{- For Hugs, use the option -F"cpp -P -traditional" -}
+
+module Pkg where
+
+import qualified Prelude
+import qualified CavaClass
+import qualified CavaPrelude
+import qualified Monad
+import qualified Nat
+import qualified Signal
+import qualified Vector
+import qualified VectorUtils
+
+#ifdef __GLASGOW_HASKELL__
+import qualified GHC.Base
+#else
+-- HUGS
+import qualified IOExts
+#endif
+
+#ifdef __GLASGOW_HASKELL__
+type Any = GHC.Base.Any
+#else
+-- HUGS
+type Any = ()
+#endif
+
+aes_transpose :: 
+(CavaClass.Cava
+a1) ->
+Prelude.Integer
+->
+Prelude.Integer
+-> a1 ->
+a1
+aes_transpose semantics n m matrix =
+  
+let {
+columns = 
+CavaClass.peel
+semantics
+(Signal.Vec
+(Signal.Vec
+Signal.Bit
+(Prelude.succ
+(Prelude.succ
+(Prelude.succ
+(Prelude.succ
+(Prelude.succ
+(Prelude.succ
+(Prelude.succ
+(Prelude.succ
+0)))))))))
+n) m
+matrix}
+in
+let {
+items = 
+Vector.map
+(CavaClass.peel
+semantics
+(Signal.Vec
+Signal.Bit
+(Prelude.succ
+(Prelude.succ
+(Prelude.succ
+(Prelude.succ
+(Prelude.succ
+(Prelude.succ
+(Prelude.succ
+(Prelude.succ
+0)))))))))
+n) m
+columns}
+in
+let {
+columns0 = 
+Vector.map
+(CavaClass.unpeel
+semantics
+(Signal.Vec
+Signal.Bit
+(Prelude.succ
+(Prelude.succ
+(Prelude.succ
+(Prelude.succ
+(Prelude.succ
+(Prelude.succ
+(Prelude.succ
+(Prelude.succ
+0)))))))))
+m) n
+(VectorUtils.transpose
+n m
+items)}
+in
+CavaClass.unpeel
+semantics
+(Signal.Vec
+(Signal.Vec
+Signal.Bit
+(Prelude.succ
+(Prelude.succ
+(Prelude.succ
+(Prelude.succ
+(Prelude.succ
+(Prelude.succ
+(Prelude.succ
+(Prelude.succ
+0)))))))))
+m) n
+columns0
+
+aes_mul2 :: 
+(CavaClass.Cava
+a1) ->
+(Monad.Monad
+(CavaClass.Coq_cava
+a1 
+Any)) ->
+a1 ->
+CavaClass.Coq_cava
+a1 
+a1
+aes_mul2 semantics monad x =
+  
+Monad.bind
+monad
+(CavaClass.xor2
+semantics
+((,)
+(CavaClass.indexConst
+semantics
+Signal.Bit
+(Prelude.succ
+(Prelude.succ
+(Prelude.succ
+(Prelude.succ
+(Prelude.succ
+(Prelude.succ
+(Prelude.succ
+(Prelude.succ
+0))))))))
+x 0)
+(CavaClass.indexConst
+semantics
+Signal.Bit
+(Prelude.succ
+(Prelude.succ
+(Prelude.succ
+(Prelude.succ
+(Prelude.succ
+(Prelude.succ
+(Prelude.succ
+(Prelude.succ
+0))))))))
+x
+(Prelude.succ
+(Prelude.succ
+(Prelude.succ
+(Prelude.succ
+(Prelude.succ
+(Prelude.succ
+(Prelude.succ
+0))))))))))
+(\a ->
+Monad.bind
+monad
+(CavaClass.xor2
+semantics
+((,)
+(CavaClass.indexConst
+semantics
+Signal.Bit
+(Prelude.succ
+(Prelude.succ
+(Prelude.succ
+(Prelude.succ
+(Prelude.succ
+(Prelude.succ
+(Prelude.succ
+(Prelude.succ
+0))))))))
+x
+(Prelude.succ
+(Prelude.succ
+0)))
+(CavaClass.indexConst
+semantics
+Signal.Bit
+(Prelude.succ
+(Prelude.succ
+(Prelude.succ
+(Prelude.succ
+(Prelude.succ
+(Prelude.succ
+(Prelude.succ
+(Prelude.succ
+0))))))))
+x
+(Prelude.succ
+(Prelude.succ
+(Prelude.succ
+(Prelude.succ
+(Prelude.succ
+(Prelude.succ
+(Prelude.succ
+0))))))))))
+(\b ->
+Monad.bind
+monad
+(CavaClass.xor2
+semantics
+((,)
+(CavaClass.indexConst
+semantics
+Signal.Bit
+(Prelude.succ
+(Prelude.succ
+(Prelude.succ
+(Prelude.succ
+(Prelude.succ
+(Prelude.succ
+(Prelude.succ
+(Prelude.succ
+0))))))))
+x
+(Prelude.succ
+(Prelude.succ
+(Prelude.succ
+0))))
+(CavaClass.indexConst
+semantics
+Signal.Bit
+(Prelude.succ
+(Prelude.succ
+(Prelude.succ
+(Prelude.succ
+(Prelude.succ
+(Prelude.succ
+(Prelude.succ
+(Prelude.succ
+0))))))))
+x
+(Prelude.succ
+(Prelude.succ
+(Prelude.succ
+(Prelude.succ
+(Prelude.succ
+(Prelude.succ
+(Prelude.succ
+0))))))))))
+(\c ->
+Monad.ret
+monad
+(CavaClass.unpeel
+semantics
+Signal.Bit
+(Prelude.succ
+(Prelude.succ
+(Prelude.succ
+(Prelude.succ
+(Prelude.succ
+(Prelude.succ
+(Prelude.succ
+(Prelude.succ
+0))))))))
+(Vector.Coq_cons
+(CavaClass.indexConst
+semantics
+Signal.Bit
+(Prelude.succ
+(Prelude.succ
+(Prelude.succ
+(Prelude.succ
+(Prelude.succ
+(Prelude.succ
+(Prelude.succ
+(Prelude.succ
+0))))))))
+x
+(Prelude.succ
+(Prelude.succ
+(Prelude.succ
+(Prelude.succ
+(Prelude.succ
+(Prelude.succ
+(Prelude.succ
+0))))))))
+(Prelude.succ
+(Prelude.succ
+(Prelude.succ
+(Prelude.succ
+(Prelude.succ
+(Prelude.succ
+(Prelude.succ
+0)))))))
+(Vector.Coq_cons
+a
+(Prelude.succ
+(Prelude.succ
+(Prelude.succ
+(Prelude.succ
+(Prelude.succ
+(Prelude.succ
+0))))))
+(Vector.Coq_cons
+(CavaClass.indexConst
+semantics
+Signal.Bit
+(Prelude.succ
+(Prelude.succ
+(Prelude.succ
+(Prelude.succ
+(Prelude.succ
+(Prelude.succ
+(Prelude.succ
+(Prelude.succ
+0))))))))
+x
+(Prelude.succ
+0))
+(Prelude.succ
+(Prelude.succ
+(Prelude.succ
+(Prelude.succ
+(Prelude.succ
+0)))))
+(Vector.Coq_cons
+b
+(Prelude.succ
+(Prelude.succ
+(Prelude.succ
+(Prelude.succ
+0))))
+(Vector.Coq_cons
+c
+(Prelude.succ
+(Prelude.succ
+(Prelude.succ
+0)))
+(Vector.Coq_cons
+(CavaClass.indexConst
+semantics
+Signal.Bit
+(Prelude.succ
+(Prelude.succ
+(Prelude.succ
+(Prelude.succ
+(Prelude.succ
+(Prelude.succ
+(Prelude.succ
+(Prelude.succ
+0))))))))
+x
+(Prelude.succ
+(Prelude.succ
+(Prelude.succ
+(Prelude.succ
+0)))))
+(Prelude.succ
+(Prelude.succ
+0))
+(Vector.Coq_cons
+(CavaClass.indexConst
+semantics
+Signal.Bit
+(Prelude.succ
+(Prelude.succ
+(Prelude.succ
+(Prelude.succ
+(Prelude.succ
+(Prelude.succ
+(Prelude.succ
+(Prelude.succ
+0))))))))
+x
+(Prelude.succ
+(Prelude.succ
+(Prelude.succ
+(Prelude.succ
+(Prelude.succ
+0))))))
+(Prelude.succ
+0)
+(Vector.Coq_cons
+(CavaClass.indexConst
+semantics
+Signal.Bit
+(Prelude.succ
+(Prelude.succ
+(Prelude.succ
+(Prelude.succ
+(Prelude.succ
+(Prelude.succ
+(Prelude.succ
+(Prelude.succ
+0))))))))
+x
+(Prelude.succ
+(Prelude.succ
+(Prelude.succ
+(Prelude.succ
+(Prelude.succ
+(Prelude.succ
+0)))))))
+0
+Vector.Coq_nil))))))))))))
+
+aes_mul4 :: 
+(CavaClass.Cava
+a1) ->
+(Monad.Monad
+(CavaClass.Coq_cava
+a1 
+Any)) ->
+a1 ->
+CavaClass.Coq_cava
+a1 
+a1
+aes_mul4 semantics monad =
+  
+Monad.mcompose
+monad
+(aes_mul2
+semantics
+monad)
+(aes_mul2
+semantics
+monad)
+
+zero_byte :: 
+(CavaClass.Cava
+a1) -> a1
+zero_byte semantics =
+  
+CavaClass.unpeel
+semantics
+Signal.Bit
+(Prelude.succ
+(Prelude.succ
+(Prelude.succ
+(Prelude.succ
+(Prelude.succ
+(Prelude.succ
+(Prelude.succ
+(Prelude.succ
+0))))))))
+(Vector.const
+(CavaPrelude.zero
+semantics)
+(Prelude.succ
+(Prelude.succ
+(Prelude.succ
+(Prelude.succ
+(Prelude.succ
+(Prelude.succ
+(Prelude.succ
+(Prelude.succ
+0)))))))))
+
+aes_circ_byte_shift :: 
+(CavaClass.Cava
+a1) ->
+(Monad.Monad
+(CavaClass.Coq_cava
+a1 
+Any)) ->
+Prelude.Integer
+-> a1 ->
+CavaClass.Coq_cava
+a1 
+a1
+aes_circ_byte_shift semantics monad shift input =
+  
+let {
+indices = Vector.Coq_cons
+(Nat.sub
+(Prelude.succ
+(Prelude.succ
+(Prelude.succ
+(Prelude.succ
+0))))
+shift)
+(Prelude.succ
+(Prelude.succ
+(Prelude.succ
+0)))
+(Vector.Coq_cons
+(Nat.sub
+(Prelude.succ
+(Prelude.succ
+(Prelude.succ
+(Prelude.succ
+(Prelude.succ
+0)))))
+shift)
+(Prelude.succ
+(Prelude.succ
+0))
+(Vector.Coq_cons
+(Nat.sub
+(Prelude.succ
+(Prelude.succ
+(Prelude.succ
+(Prelude.succ
+(Prelude.succ
+(Prelude.succ
+0))))))
+shift)
+(Prelude.succ
+0)
+(Vector.Coq_cons
+(Nat.sub
+(Prelude.succ
+(Prelude.succ
+(Prelude.succ
+(Prelude.succ
+(Prelude.succ
+(Prelude.succ
+(Prelude.succ
+0)))))))
+shift) 0
+Vector.Coq_nil)))}
+in
+let {
+indices0 = 
+Vector.map
+(\x ->
+Nat.modulo
+x
+(Prelude.succ
+(Prelude.succ
+(Prelude.succ
+(Prelude.succ
+0)))))
+(Prelude.succ
+(Prelude.succ
+(Prelude.succ
+(Prelude.succ
+0))))
+indices}
+in
+Monad.ret
+monad
+(CavaClass.unpeel
+semantics
+(Signal.Vec
+Signal.Bit
+(Prelude.succ
+(Prelude.succ
+(Prelude.succ
+(Prelude.succ
+(Prelude.succ
+(Prelude.succ
+(Prelude.succ
+(Prelude.succ
+0)))))))))
+(Prelude.succ
+(Prelude.succ
+(Prelude.succ
+(Prelude.succ
+0))))
+(Vector.map
+(CavaClass.indexConst
+semantics
+(Signal.Vec
+Signal.Bit
+(Prelude.succ
+(Prelude.succ
+(Prelude.succ
+(Prelude.succ
+(Prelude.succ
+(Prelude.succ
+(Prelude.succ
+(Prelude.succ
+0)))))))))
+(Prelude.succ
+(Prelude.succ
+(Prelude.succ
+(Prelude.succ
+0))))
+input)
+(Prelude.succ
+(Prelude.succ
+(Prelude.succ
+(Prelude.succ
+0))))
+indices0))
+
