investigations/extraction/ExtractionTests.hs
@@ -1,0 +1,55 @@
+module ExtractionTests where
+
+import qualified Prelude
+import qualified BinNums
+
+wombat_nat :: ([]) Prelude.Integer
+wombat_nat =
+  (:) (Prelude.succ (Prelude.succ (Prelude.succ (Prelude.succ (Prelude.succ
+    (Prelude.succ (Prelude.succ (Prelude.succ (Prelude.succ (Prelude.succ
+    (Prelude.succ (Prelude.succ (Prelude.succ 0))))))))))))) ((:)
+    (Prelude.succ (Prelude.succ (Prelude.succ (Prelude.succ (Prelude.succ
+    (Prelude.succ (Prelude.succ (Prelude.succ (Prelude.succ (Prelude.succ
+    (Prelude.succ (Prelude.succ (Prelude.succ (Prelude.succ (Prelude.succ
+    (Prelude.succ (Prelude.succ (Prelude.succ (Prelude.succ (Prelude.succ
+    (Prelude.succ (Prelude.succ (Prelude.succ (Prelude.succ (Prelude.succ
+    (Prelude.succ (Prelude.succ (Prelude.succ (Prelude.succ (Prelude.succ
+    (Prelude.succ (Prelude.succ (Prelude.succ (Prelude.succ (Prelude.succ
+    (Prelude.succ (Prelude.succ (Prelude.succ (Prelude.succ (Prelude.succ
+    (Prelude.succ (Prelude.succ 0))))))))))))))))))))))))))))))))))))))))))
+    ((:) (Prelude.succ (Prelude.succ (Prelude.succ (Prelude.succ
+    (Prelude.succ (Prelude.succ (Prelude.succ (Prelude.succ (Prelude.succ
+    (Prelude.succ (Prelude.succ (Prelude.succ (Prelude.succ 0)))))))))))))
+    ((:) (Prelude.succ (Prelude.succ (Prelude.succ (Prelude.succ
+    (Prelude.succ (Prelude.succ (Prelude.succ (Prelude.succ (Prelude.succ
+    (Prelude.succ (Prelude.succ (Prelude.succ (Prelude.succ (Prelude.succ
+    (Prelude.succ (Prelude.succ (Prelude.succ (Prelude.succ (Prelude.succ
+    (Prelude.succ (Prelude.succ (Prelude.succ (Prelude.succ (Prelude.succ
+    (Prelude.succ (Prelude.succ (Prelude.succ (Prelude.succ (Prelude.succ
+    (Prelude.succ (Prelude.succ (Prelude.succ (Prelude.succ (Prelude.succ
+    (Prelude.succ (Prelude.succ (Prelude.succ (Prelude.succ (Prelude.succ
+    (Prelude.succ (Prelude.succ (Prelude.succ (Prelude.succ (Prelude.succ
+    (Prelude.succ (Prelude.succ (Prelude.succ (Prelude.succ (Prelude.succ
+    (Prelude.succ (Prelude.succ (Prelude.succ (Prelude.succ (Prelude.succ
+    (Prelude.succ (Prelude.succ (Prelude.succ (Prelude.succ (Prelude.succ
+    (Prelude.succ (Prelude.succ (Prelude.succ (Prelude.succ (Prelude.succ
+    (Prelude.succ (Prelude.succ (Prelude.succ (Prelude.succ (Prelude.succ
+    (Prelude.succ (Prelude.succ (Prelude.succ (Prelude.succ (Prelude.succ
+    (Prelude.succ (Prelude.succ (Prelude.succ (Prelude.succ (Prelude.succ
+    (Prelude.succ (Prelude.succ (Prelude.succ (Prelude.succ
+    0)))))))))))))))))))))))))))))))))))))))))))))))))))))))))))))))))))))))))))))))))))
+    ([]))))
+
+numbat_nat :: ([]) BinNums.N
+numbat_nat =
+  (:) (BinNums.Npos ((\x -> 2 Prelude.* x) ((\x -> 2 Prelude.* x Prelude.+ 1)
+    ((\x -> 2 Prelude.* x Prelude.+ 1) ((\x -> 2 Prelude.* x)
+    ((\x -> 2 Prelude.* x Prelude.+ 1) ((\x -> 2 Prelude.* x) 1))))))) ((:)
+    (BinNums.Npos ((\x -> 2 Prelude.* x) ((\x -> 2 Prelude.* x Prelude.+ 1)
+    ((\x -> 2 Prelude.* x) ((\x -> 2 Prelude.* x Prelude.+ 1)
+    ((\x -> 2 Prelude.* x Prelude.+ 1) ((\x -> 2 Prelude.* x) 1))))))) ((:)
+    (BinNums.Npos ((\x -> 2 Prelude.* x) ((\x -> 2 Prelude.* x) 1))) ((:)
+    (BinNums.Npos ((\x -> 2 Prelude.* x Prelude.+ 1)
+    ((\x -> 2 Prelude.* x Prelude.+ 1) ((\x -> 2 Prelude.* x)
+    ((\x -> 2 Prelude.* x) ((\x -> 2 Prelude.* x Prelude.+ 1) 1)))))) ([]))))
+
